\documentclass[a4paper,12pt]{article}
\usepackage{amsmath}
\usepackage{amssymb}
\begin{document}
\setlength\parindent{0pt}
\textbf{Project Euler 512}
\vspace{5ex}

\(\sum_{i = 1}^n \varphi (n^i) = \sum_{i = 1}^n n^{i - 1} \varphi (n) = \varphi(n) (1 + n + \dots + n^{n - 1})\)

We can group \(1 + n + \dots + n^{n - 1}\) as either \((1+n)(1 + n^2 + \dots + n^{n - 2})\) or \(1 + (1 + n)(n + n^3 + \dots + n^{n - 2})\), so \(f(n) = 0\) if \(n\) is even and \(f(n) = \varphi(n)\) otherwise.
\end{document}